src/program_proof/examples/dir_proof.v
@@ -1,1 +1,155 @@
+From Perennial.Helpers Require Import Map.
+
 From Goose.github_com.mit_pdos.perennial_examples Require Import dir.
+From Perennial.program_proof Require Import proof_prelude.
+From Perennial.goose_lang.lib Require Import into_val.
+
+Instance unit_IntoVal : IntoVal ().
+Proof.
+  refine {| to_val := λ _, #();
+            IntoVal_def := ();
+         |}.
+  intros [] [] _; auto.
+Defined.
+
+Instance unit_IntoValForType : IntoValForType unit_IntoVal (struct.t unit.S).
+Proof.
+  constructor; auto.
+Qed.
+
+Section goose.
+Context `{!heapG Σ}.
+
+Implicit Types (free: gmap u64 ()).
+
+Theorem wp_FreeRange (start sz: u64) :
+  int.val start + int.val sz < 2^64 ->
+  {{{ True }}}
+    FreeRange #start #sz
+  {{{ (mref: loc) free, RET #mref;
+      is_map mref free ∗
+      ⌜∀ (x:u64), int.val start ≤ int.val x < int.val start + int.val sz ->
+                  free !! x = Some tt⌝ }}}.
+Proof.
+  iIntros (Hbound Φ) "_ HΦ".
+  wp_call.
+  wp_apply (wp_NewMap () (t:=struct.t unit.S)).
+  iIntros (mref) "Hmap".
+  wp_apply wp_ref_to; first by val_ty.
+  iIntros (il) "i".
+  wp_pures.
+  wp_apply (wp_forUpto (λ i, ∃ free, "Hmap" ∷ is_map mref free ∗
+      "%Hmap_vals" ∷ ⌜∀ (x:u64), int.val start ≤ int.val x < int.val i ->
+                      free !! x = Some tt⌝)%I
+            with "[] [Hmap $i]").
+  - word.
+  - clear Φ.
+    iIntros (i).
+    iIntros "!>" (Φ) "(HI & i & %Hibound) HΦ"; iNamed "HI".
+    wp_pures.
+    wp_load.
+    wp_apply (wp_MapInsert _ _ _ _ () with "Hmap"); auto.
+    iIntros "Hm".
+    wp_pures.
+    iApply "HΦ".
+    iFrame.
+    iExists _; iFrame.
+    iPureIntro.
+    replace (int.val (word.add i 1)) with (int.val i + 1) by word.
+    intros x Hxbound.
+    destruct (decide (x = i)); subst.
+    + rewrite lookup_insert //.
+    + rewrite lookup_insert_ne //.
+      apply Hmap_vals.
+      assert (int.val x ≠ int.val i) by (apply not_inj; auto).
+      word.
+  - iExists _; iFrame.
+    iPureIntro.
+    intros x Hxbound.
+    word.
+  - iIntros "[HI i]"; iNamed "HI".
+    wp_pures.
+    iApply "HΦ"; iFrame.
+    iPureIntro.
+    intros.
+    apply Hmap_vals.
+    word.
+Qed.
+
+Lemma big_sepM_lookup_holds {PROP:bi} `{Countable K} {V} (m: gmap K V) :
+  ⊢@{PROP} [∗ map] k↦v ∈ m, ⌜m !! k = Some v⌝.
+Proof.
+  rewrite big_opM_eq /big_opM_def /curry /=.
+  assert (map_Forall (λ (k:K) (v:V), m !! k = Some v) m) as Hmap.
+  { apply map_Forall_lookup; auto. }
+  apply map_Forall_to_list in Hmap.
+  generalize dependent (map_to_list m).
+  induction l as [|kv kvs IH]; simpl; intros; auto.
+  inversion Hmap; subst.
+  destruct kv as [k v].
+  iSplitL.
+  + simpl in H3; auto.
+  + intuition.
+Qed.
+
+Lemma big_sepM_lookup_unit (PROP:bi) `{Countable K} (m: gmap K ()) :
+  ⊢@{PROP} [∗ map] k↦_ ∈ m, ⌜m !! k = Some tt⌝.
+Proof.
+  iDestruct (big_sepM_lookup_holds m) as "Hmap".
+  iApply (big_sepM_mono with "Hmap"); simpl; intros.
+  destruct x; auto.
+Qed.
+
+Theorem wp_findKey mref free :
+  {{{ is_map mref free }}}
+    findKey #mref
+  {{{ (k: u64) (ok: bool), RET (#k, #ok);
+      ⌜if ok then free !! k = Some tt else True⌝ ∗
+      is_map mref free
+  }}}.
+Proof.
+  iIntros (Φ) "Hmap HΦ".
+  wp_call.
+  wp_apply wp_ref_to; first by val_ty.
+  iIntros (found_l) "found".
+  wp_apply wp_ref_to; first by val_ty.
+  iIntros (ok_l) "ok".
+  wp_pures.
+  wp_apply (wp_MapIter _ _ _ _
+                       (∃ (found: u64) (ok: bool),
+                           "found" ∷ found_l ↦[uint64T] #found ∗
+                           "ok" ∷ ok_l ↦[boolT] #ok ∗
+                           "%Hfound_is" ∷ ⌜if ok then free !! found = Some tt else True⌝)
+                       (λ k _, ⌜free !! k = Some tt⌝)%I
+                       (λ _ _, True)%I
+                       with "Hmap [found ok]").
+  - iExists _, _; iFrame.
+  - (* TODO: should be able to prove this with iPureIntro and then something
+    simple, but there's no IntoPure for big_sepM *)
+    iApply big_sepM_lookup_unit.
+  - iIntros (k v) "!>".
+    clear Φ.
+    iIntros (Φ) "[HI %Helem] HΦ"; iNamed "HI".
+    wp_pures.
+    wp_load.
+    wp_pures.
+    wp_if_destruct.
+    + wp_store. wp_store.
+      iApply "HΦ".
+      iSplitL; auto.
+      iExists _, _; iFrame.
+      auto.
+    + iApply "HΦ".
+      iSplitL; auto.
+      iExists _, _; iFrame.
+      apply negb_false_iff in Heqb; subst.
+      auto.
+  - iIntros "(His_map&HI&_HQ)"; iNamed "HI".
+    wp_pures.
+    wp_load. wp_load.
+    wp_pures.
+    iApply "HΦ"; iFrame.
+    auto.
+Qed.
+
+End goose.
